CoqOfRust/core/fmt/links/mod.v
@@ -55,3 +55,4 @@ Module Impl_Arguments.
     run_symbolic.
   Admitted.
 End Impl_Arguments.
+Export Impl_Arguments.
