CoqOfRust/core/simulations/tuple.v
@@ -1,8 +1,6 @@
 Require Import CoqOfRust.CoqOfRust.
 Require Import simulations.M.
-Import simulations.M.Notations.
 Require Import CoqOfRust.core.simulations.eq.
-Import simulations.eq.Notations.
 
 Module ImplEq.
   Global Instance I (A B : Set) `{Eq.Trait A} `{Eq.Trait B} :
