CoqOfRust/links/M.v
@@ -1,9 +1,5 @@
 Require Import CoqOfRust.CoqOfRust.
 
-Import List.ListNotations.
-
-Local Open Scope list.
-
 Axiom IsTraitAssociatedType_eq :
   forall
     (trait_name : string)
