CoqOfRust/move_sui/simulations/move_binary_format/lib.v
@@ -2,8 +2,6 @@ Require Import CoqOfRust.CoqOfRust.
 Require Import CoqOfRust.simulations.M.
 Require Import CoqOfRust.lib.lib.
 
-Import simulations.M.Notations.
-
 Module IndexKind.
   Inductive t : Set :=
   | ModuleHandle
