CoqOfRust/move_sui/simulations/move_bytecode_verifier_meter/lib.v
@@ -1,9 +1,6 @@
 Require Import CoqOfRust.CoqOfRust.
 Require Import CoqOfRust.simulations.M.
 Require Import CoqOfRust.lib.lib.
-
-Import simulations.M.Notations.
-
 Require CoqOfRust.move_sui.simulations.move_binary_format.errors.
 Module PartialVMResult := errors.PartialVMResult.
 Module PartialVMError := errors.PartialVMError.
