CoqOfRust/revm/revm_interpreter/instructions/links/tx_info.v
@@ -20,17 +20,6 @@ Require Import revm.revm_interpreter.links.interpreter_types.
 Require Import revm.revm_specification.links.hardfork.
 Require Import ruint.links.from.
 
-Import Impl_Gas.
-Import Impl_Option.
-Import Impl_Result_T_E.
-Import Impl_Slice.
-Import Impl_SliceIndex_for_Usize.
-Import Impl_SpecId.
-Import from.Impl_Uint.
-Import lib.Impl_Uint.
-Import Impl_u64.
-Import Impl_usize.
-
 (*
 pub fn gasprice<WIRE: InterpreterTypes, H: Host + ?Sized>(
     interpreter: &mut Interpreter<WIRE>,
