CoqOfRust/ruint/links/bits.v
@@ -1,0 +1,19 @@
+Require Import CoqOfRust.CoqOfRust.
+Require Import links.M.
+Require Import ruint.links.lib.
+Require Import ruint.bits.
+
+Module Impl_Uint.
+  Definition Self (BITS LIMBS : Usize.t) : Set :=
+    Uint.t BITS LIMBS.
+
+  (* pub const fn bit(&self, index: usize) -> bool *)
+  Instance run_bit (BITS LIMBS : Usize.t)
+      (self : Ref.t Pointer.Kind.Ref (Self BITS LIMBS))
+      (index : Usize.t) :
+    Run.Trait
+      (bits.Impl_ruint_Uint_BITS_LIMBS.bit (φ BITS) (φ LIMBS)) [] [] [ φ self; φ index ]
+      bool.
+  Admitted.
+End Impl_Uint.
+Export Impl_Uint.
